Hybrid_Programs/Proof_Automation.thy
@@ -240,7 +240,7 @@ text \<open> A first attempt at a high-level automated proof strategy using diff
 
 method dDiscr = (rule_tac nmods_invariant[OF nmods_g_orbital_on_discrete']; unrest)
 
-method dInduct = (subst dInduct_hoare_diff_inv_on fbox_diff_inv_on; 
+method dInduct = (subst hoare_diff_inv_on' fbox_diff_inv_on; 
     rule_tac lderiv_rules; 
     simp add: framed_derivs ldifferentiable closure usubst unrest_ssubst unrest usubst_eval)
 
